Canonical structure-based AT, DOT syntax

theories/lang/cpp/logic/rep.v
@@ -9,65 +9,16 @@ Require Import iris.bi.lib.fractional.
 
 Require Import bedrock.prelude.base.
 
-From bedrock.lang.cpp Require Import semantics.values logic.mpred.
+From bedrock.lang.cpp Require Import semantics.values logic.mpred logic.rep_defs heap_notations.
 From bedrock.lang.bi Require Import prelude only_provable observe laterable.
 
 Import ChargeNotation.
 Implicit Types (σ resolve : genv) (p : ptr) (o : offset).
 
-(** representations are predicates over a location, they should be used to
-  * assert properties of the heap
-  *)
-Canonical Structure ptr_bi_index : biIndex :=
-  BiIndex ptr _ eq _.
-
-(** The tactic [intros ->%ptr_rel_elim] is much faster than [intros
-    ->] when introducing [p1 ⊑ p2] (when the latter works at all). *)
-Lemma ptr_rel_elim (p1 p2 : ptr) : p1 ⊑ p2 → p1 = p2.
-Proof. done. Qed.
-
-Definition Rep `{Σ : cpp_logic} := monPred ptr_bi_index mpredI.
-Canonical Structure RepI `{Σ : cpp_logic} := monPredI ptr_bi_index mpredI.
-Canonical Structure RepO `{Σ : cpp_logic} := monPredO ptr_bi_index mpredI.
-
-Bind Scope bi_scope with Rep.
-
-Section defs.
-  Context `{Σ : cpp_logic}.
-
-  Definition as_Rep (P : ptr -> mpred) : Rep := MonPred P _.
-
-  (** [_at base R] states that [R base] holds.
-
-      NOTE This is "weakly at"
-   *)
-  Definition _at_def (base : ptr) (R : Rep) : mpred :=
-    R.(monPred_at) base.
-  Definition _at_aux : seal (@_at_def). Proof. by eexists. Qed.
-  Definition _at := _at_aux.(unseal).
-  Definition _at_eq : @_at = _ := _at_aux.(seal_eq).
-
-  Definition _offsetR_def (o : offset) (r : Rep) : Rep :=
-    as_Rep (fun base => r.(monPred_at) (_offset_ptr base o)).
-  Definition _offsetR_aux : seal (@_offsetR_def). Proof. by eexists. Qed.
-  Definition _offsetR := _offsetR_aux.(unseal).
-  Definition _offsetR_eq : @_offsetR = _ := _offsetR_aux.(seal_eq).
-
-  (** Values
-   * These `Rep` predicates wrap `ptsto` facts
-   *)
-  (* todo(gmm): make opaque *)
-  Definition pureR (P : mpred) : Rep :=
-    as_Rep (fun _ => P).
-End defs.
-
-#[global] Instance: Params (@_at) 3 := {}.
-#[global] Instance: Params (@as_Rep) 2 := {}.
-#[global] Instance: Params (@_offsetR) 3 := {}.
-#[global] Instance: Params (@pureR) 2 := {}.
-
 Section with_cpp.
   Context `{Σ : cpp_logic}.
+
+  Implicit Type (R : Rep).
 
   (** See also [Rep_equiv_at] and [Rep_entails_at]. *)
   Lemma Rep_ext (P Q : Rep) :
@@ -219,164 +170,169 @@ Section with_cpp.
     (P ∗-∗ Q) p ⊣⊢ (P p ∗-∗ Q p).
   Proof. by rewrite /bi_wand_iff monPred_at_and !Rep_wand_force. Qed.
 
+  Import heap_notations.INTERNAL.
+
   #[global] Instance _offsetR_ne o n : Proper (dist n ==> dist n) (_offsetR o).
-  Proof. rewrite _offsetR_eq. solve_proper. Qed.
+  Proof. unfold_at. solve_proper. Qed.
   #[global] Instance _offsetR_proper o : Proper ((≡) ==> (≡)) (_offsetR o).
-  Proof. rewrite _offsetR_eq. solve_proper. Qed.
+  Proof. unfold_at. solve_proper. Qed.
   #[global] Instance _offsetR_mono o : Proper ((⊢) ==> (⊢)) (_offsetR o).
-  Proof. rewrite _offsetR_eq. solve_proper. Qed.
+  Proof. unfold_at. solve_proper. Qed.
   #[local] Lemma _offsetR_mono_old : Proper (eq ==> (⊢) ==> (⊢)) _offsetR.
-  Proof. solve_proper. Qed.
+  Proof. unfold_at. solve_proper. Qed.
   #[global] Instance _offsetR_flip_mono o : Proper (flip (⊢) ==> flip (⊢)) (_offsetR o).
-  Proof. rewrite _offsetR_eq. solve_proper. Qed.
+  Proof. unfold_at. solve_proper. Qed.
 
-  #[global] Instance _offsetR_persistent o (r : Rep) :
-    Persistent r -> Persistent (_offsetR o r).
+  #[global] Instance _offsetR_persistent o (r : Rep) : Persistent r -> Persistent (o |-> r).
   Proof. rewrite _offsetR_eq. apply _. Qed.
-  #[global] Instance _offsetR_affine o (r : Rep) :
-    Affine r -> Affine (_offsetR o r).
+  #[global] Instance _offsetR_affine o (r : Rep) : Affine r -> Affine (o |-> r).
   Proof. rewrite _offsetR_eq. apply _. Qed.
-  #[global] Instance _offsetR_timeless o (r : Rep) :
-    Timeless r → Timeless (_offsetR o r).
+  #[global] Instance _offsetR_timeless o (r : Rep) : Timeless r → Timeless (o |-> r).
   Proof. rewrite _offsetR_eq. apply _. Qed.
-  #[global] Instance _offsetR_laterable o (r : Rep) :
-    Laterable r → Laterable (_offsetR o r).
+  #[global] Instance _offsetR_laterable o (r : Rep) : Laterable r → Laterable (o |-> r).
   Proof. rewrite _offsetR_eq. apply _. Qed.
 
-  Lemma _offsetR_offsetR (o1 o2 : offset) R :
-    _offsetR o1 (_offsetR o2 R) -|- _offsetR (o_dot o1 o2) R.
+  Lemma _offsetR_offsetR (o1 o2 : offset) R : o1 |-> (o2 |-> R) -|- o1 ,, o2 |-> R.
   Proof.
-    rewrite _offsetR_eq/_offsetR_def/=.
+    rewrite !_offsetR_eq/_offsetR_def/=.
     f_equiv. by intro; rewrite offset_ptr_dot.
   Qed.
 
-  Lemma _offsetR_emp o : _offsetR o emp ⊣⊢ emp.
+  Lemma _offsetR_emp o : o |-> emp ⊣⊢ emp.
   Proof.
     rewrite _offsetR_eq /_offsetR_def.
     constructor=> p /=. by rewrite !monPred_at_emp.
   Qed.
   Lemma _offsetR_sep o r1 r2 :
-    _offsetR o (r1 ** r2) -|- _offsetR o r1 ** _offsetR o r2.
+    o |-> (r1 ** r2) -|- o |-> r1 ** o |-> r2.
   Proof.
-    rewrite _offsetR_eq /_offsetR_def -as_Rep_sep.
+    rewrite !_offsetR_eq /_offsetR_def -as_Rep_sep.
     constructor=> p /=. by rewrite monPred_at_sep.
   Qed.
   Lemma _offsetR_pure (o : offset) (P : Prop) :
-    _offsetR o (bi_pure P) -|- bi_pure P.
+    o |-> (bi_pure P) -|- bi_pure P.
   Proof.
     rewrite _offsetR_eq/_offsetR_def /=.
     by constructor=> p/=; rewrite !monPred_at_pure.
   Qed.
 
   Lemma _offsetR_only_provable (o : offset) (P : Prop) :
-    _offsetR o [| P |] -|- [| P |].
+    o |-> [| P |] -|- [| P |].
   Proof.
     rewrite _offsetR_eq/_offsetR_def /=.
     by constructor=> p/=; rewrite !monPred_at_only_provable.
   Qed.
 
   Lemma _offsetR_and (o : offset) P Q :
-    _offsetR o (P //\\ Q) -|- _offsetR o P //\\ _offsetR o Q.
+    o |-> (P //\\ Q) -|- o |-> P //\\ o |-> Q.
   Proof.
-    rewrite _offsetR_eq/_offsetR_def /=.
+    rewrite !_offsetR_eq/_offsetR_def /=.
     by constructor=> p/=; rewrite !monPred_at_and.
   Qed.
 
   Lemma _offsetR_or (o : offset) P Q :
-    _offsetR o (P \\// Q) -|- _offsetR o P \\// _offsetR o Q.
+    o |-> (P \\// Q) -|- o |-> P \\// o |-> Q.
   Proof.
-    rewrite _offsetR_eq/_offsetR_def /=.
+    rewrite !_offsetR_eq/_offsetR_def /=.
     by constructor=> p/=; rewrite !monPred_at_or.
   Qed.
 
   Lemma _offsetR_wand o (P Q : Rep) :
-      _offsetR o (P -* Q) -|- _offsetR o P -* _offsetR o Q.
+      o |-> (P -* Q) -|- o |-> P -* o |-> Q.
   Proof.
-    rewrite !_offsetR_eq /_offsetR_def /=.
+    rewrite /= !_offsetR_eq /_offsetR_def /=.
     constructor=> p/=. by rewrite !Rep_wand_force.
   Qed.
 
   Lemma _offsetR_exists o {T} (P : T -> Rep) :
-      _offsetR o (Exists v : T, P v) -|- Exists v, _offsetR o (P v).
-  Proof. by rewrite _offsetR_eq/_offsetR_def /as_Rep/=; constructor =>p; rewrite /= !monPred_at_exist. Qed.
+      o |-> (Exists v : T, P v) -|- Exists v, o |-> (P v).
+  Proof.
+    rewrite _offsetR_eq /_offsetR_def /as_Rep/=.
+    constructor =>p; rewrite /= !monPred_at_exist.
+    by iSplit; iIntros "H"; iDestruct "H" as (x) "H"; iExists x; rewrite _offsetR_eq.
+  Qed.
 
   Lemma _offsetR_forall o T (P : T -> Rep) :
-    _offsetR o (Forall x, P x) -|- Forall x, _offsetR o (P x).
-  Proof. by rewrite _offsetR_eq/_offsetR_def /as_Rep/=; constructor =>p; rewrite /= !monPred_at_forall. Qed.
+    o |-> (Forall x, P x) -|- Forall x, o |-> (P x).
+  Proof.
+    rewrite _offsetR_eq /as_Rep/=.
+    constructor =>p; rewrite /= !monPred_at_forall.
+    by iSplit; iIntros "H" (x); iSpecialize ("H" $! x); rewrite _offsetR_eq.
+  Qed.
 
-  Lemma _offsetR_pers o R : _offsetR o (<pers> R) -|- <pers> _offsetR o R.
-  Proof. by rewrite !_offsetR_eq /_offsetR_def /=; constructor=> p/=; rewrite !monPred_at_persistently. Qed.
+  Lemma _offsetR_pers o R : o |-> (<pers> R) -|- <pers> o |-> R.
+  Proof. rewrite !_offsetR_eq. by constructor=> p/=; rewrite !monPred_at_persistently. Qed.
 
-  Lemma _offsetR_bupd o R : _offsetR o (|==> R) -|- |==> _offsetR o R.
-  Proof. by rewrite _offsetR_eq/_offsetR_def /as_Rep; constructor => p /=; rewrite !monPred_at_bupd. Qed.
+  Lemma _offsetR_bupd o R : o |-> (|==> R) -|- |==> o |-> R.
+  Proof. by rewrite !_offsetR_eq /as_Rep; constructor => p /=; rewrite !monPred_at_bupd. Qed.
 
-  Lemma _offsetR_fupd o R E1 E2 : _offsetR o (|={E1,E2}=> R) -|- |={E1,E2}=> _offsetR o R.
-  Proof. by rewrite _offsetR_eq/_offsetR_def /as_Rep; constructor => p /=; rewrite !monPred_at_fupd. Qed.
+  Lemma _offsetR_fupd o R E1 E2 : o |-> (|={E1,E2}=> R) -|- |={E1,E2}=> o |-> R.
+  Proof. by rewrite !_offsetR_eq /as_Rep; constructor => p /=; rewrite !monPred_at_fupd. Qed.
 
-  Lemma _offsetR_intuitionistically o (R : Rep) : _offsetR o (□ R) ⊣⊢ □ (_offsetR o R).
-  Proof. by rewrite _offsetR_eq/_offsetR_def; constructor => p /=; rewrite !monPred_at_intuitionistically. Qed.
+  Lemma _offsetR_intuitionistically o (R : Rep) : o |-> (□ R) ⊣⊢ □ (o |-> R).
+  Proof. by rewrite !_offsetR_eq; constructor => p /=; rewrite !monPred_at_intuitionistically. Qed.
 
-  Lemma _offsetR_intuitionistically_if o b R : _offsetR o (□?b R) -|- □?b (_offsetR o R).
-  Proof. by destruct b => //=; rewrite _offsetR_intuitionistically. Qed.
+  Lemma _offsetR_intuitionistically_if o b R : o |-> (□?b R) -|- □?b (o |-> R).
+  Proof. by destruct b => //=; rewrite /= _offsetR_intuitionistically. Qed.
 
-  Lemma _offsetR_except_0 o R : _offsetR o (bi_except_0 R) -|- bi_except_0 (_offsetR o R).
-  Proof. by rewrite _offsetR_eq/_offsetR_def; constructor => p /=; rewrite !monPred_at_except_0. Qed.
+  Lemma _offsetR_except_0 o R : o |-> (bi_except_0 R) -|- bi_except_0 (o |-> R).
+  Proof. by rewrite !_offsetR_eq; constructor => p /=; rewrite !monPred_at_except_0. Qed.
 
-  Lemma _offsetR_affinely (o : offset) R : _offsetR o (<affine> R) -|- <affine> _offsetR o R.
-  Proof. by rewrite _offsetR_eq/_offsetR_def /as_Rep; constructor => p/=; rewrite !monPred_at_affinely. Qed.
+  Lemma _offsetR_affinely (o : offset) R : o |-> (<affine> R) -|- <affine> o |-> R.
+  Proof. by rewrite !_offsetR_eq /as_Rep; constructor => p/=; rewrite !monPred_at_affinely. Qed.
 
-  Lemma _offsetR_affinely_if b (o : offset) R : _offsetR o (<affine>?b R) -|- <affine>?b _offsetR o R.
+  Lemma _offsetR_affinely_if b (o : offset) R : o |-> (<affine>?b R) -|- <affine>?b o |-> R.
   Proof. by destruct b => //; rewrite _offsetR_affinely. Qed.
 
-
   Lemma _offsetR_big_sepL (o : offset) {T} (Rs : list T) : forall F,
-    _offsetR o ([∗list] i ↦ x ∈ Rs , F i x) -|- [∗list] i ↦ x ∈ Rs , _offsetR o (F i x).
+    o |-> ([∗list] i ↦ x ∈ Rs , F i x) -|- [∗list] i ↦ x ∈ Rs , o |-> (F i x).
   Proof.
     induction Rs; simpl; intros.
     - by rewrite _offsetR_emp.
     - by rewrite _offsetR_sep IHRs.
   Qed.
 
-  Lemma _offsetR_later o R : _offsetR o (|> R) -|- |> _offsetR o R.
+  Lemma _offsetR_later o R : o |-> (|> R) -|- |> o |-> R.
   Proof.
-    rewrite _offsetR_eq /_offsetR_def.
-    constructor=>p/=. by rewrite !monPred_at_later.
+    rewrite !_offsetR_eq. constructor=>p/=. by rewrite !monPred_at_later.
   Qed.
 
   #[global] Instance _offsetR_fractional o (r : Qp → Rep) :
-    Fractional r → Fractional (λ q, _offsetR o (r q)).
-  Proof. intros ? q1 q2. by rewrite fractional _offsetR_sep. Qed.
+    Fractional r → Fractional (λ q, o |-> r q).
+  Proof. by move => H q1 q2; rewrite fractional _offsetR_sep. Qed.
   #[global] Instance _offsetR_as_fractional o (r : Qp → Rep) q :
-    Fractional r → AsFractional (_offsetR o (r q)) (λ q, _offsetR o (r q)) q.
+    Fractional r → AsFractional (o |-> (r q)) (λ q, o |-> (r q)) q.
   Proof. constructor. done. apply _. Qed.
 
   #[global] Instance _offsetR_observe {o} {Q R : Rep} :
     Observe Q R ->
-    Observe (_offsetR o Q) (_offsetR o R).
-  Proof. move->. by rewrite /Observe _offsetR_pers. Qed.
+    Observe (o |-> Q) (o |-> R).
+  Proof. move->. by rewrite /Observe -_offsetR_pers. Qed.
 
   #[global] Instance _offsetR_observe_2 {o} {Q R1 R2 : Rep} :
     Observe2 Q R1 R2 ->
-    Observe2 (_offsetR o Q) (_offsetR o R1) (_offsetR o R2).
-  Proof. move->. by rewrite /Observe2 _offsetR_wand _offsetR_pers. Qed.
+    Observe2 (o |-> Q) (o |-> R1) (o |-> R2).
+  Proof.
+    rewrite /Observe2.
+    move->. by rewrite /Observe2 _offsetR_wand _offsetR_pers. Qed.
 
   #[global] Instance _offsetR_observe_only_provable Q o (R : Rep) :
-    Observe [| Q |] R → Observe [| Q |] (_offsetR o R).
+    Observe [| Q |] R → Observe [| Q |] (o |-> R).
   Proof. rewrite -{2}_offsetR_only_provable. apply _. Qed.
   #[global] Instance _offsetR_observe_2_only_provable Q o (R1 R2 : Rep) :
-    Observe2 [| Q |] R1 R2 → Observe2 [| Q |] (_offsetR o R1) (_offsetR o R2).
+    Observe2 [| Q |] R1 R2 → Observe2 [| Q |] (o |-> R1) (o |-> R2).
   Proof. rewrite -{2}_offsetR_only_provable. apply _. Qed.
 
   #[global] Instance _offsetR_observe_pure Q o (R : Rep) :
-    Observe [! Q !] R → Observe [! Q !] (_offsetR o R).
+    Observe [! Q !] R → Observe [! Q !] (o |-> R).
   Proof. rewrite -{2}_offsetR_pure. apply _. Qed.
   #[global] Instance _offsetR_observe_2_pure Q o (R1 R2 : Rep) :
-    Observe2 [! Q !] R1 R2 → Observe2 [! Q !] (_offsetR o R1) (_offsetR o R2).
+    Observe2 [! Q !] R1 R2 → Observe2 [! Q !] (o |-> R1) (o |-> R2).
   Proof. rewrite -{2}_offsetR_pure. apply _. Qed.
 
   Lemma _offsetR_obs o r P :
     r |-- r ** [| P |] →
-    _offsetR o r |-- _offsetR o r ** [| P |].
+    o |-> r |-- o |-> r ** [| P |].
   Proof.
     intros. apply observe_elim, _offsetR_observe_only_provable. exact: observe_intro.
   Qed.
@@ -390,20 +346,20 @@ Section with_cpp.
   Qed.
 
   Lemma _offsetR_dot (o1 o2 : offset) (R : Rep) :
-    _offsetR o1 (_offsetR o2 R) -|- _offsetR (o_dot o1 o2) R.
+    _offsetR o1 (_offsetR o2 R) -|- _offsetR (o1 ,, o2) R.
   Proof.
     constructor =>p/=.
-    by rewrite _offsetR_eq/_offsetR_def/= offset_ptr_dot.
+    by rewrite !_offsetR_eq/= offset_ptr_dot.
   Qed.
 
-  #[global] Instance _at_ne l {n} : Proper (dist n ==> dist n) (_at l).
-  Proof. rewrite _at_eq. solve_proper. Qed.
+  #[global] Instance _at_ne p {n} : Proper (dist n ==> dist n) (_at p).
+  Proof. unfold_at. solve_proper. Qed.
   #[global] Instance _at_proper {p} : Proper ((≡) ==> (≡)) (_at p).
-  Proof. rewrite _at_eq. solve_proper. Qed.
+  Proof. unfold_at. solve_proper. Qed.
   #[global] Instance _at_mono {p} : Proper ((⊢) ==> (⊢)) (_at p).
-  Proof. rewrite _at_eq. solve_proper. Qed.
+  Proof. unfold_at. solve_proper. Qed.
   #[global] Instance _at_flip_mono {p} : Proper (flip (⊢) ==> flip (⊢)) (_at p).
-  Proof. rewrite _at_eq/_at_def=> r1 r2 HR/=. by rewrite HR. Qed.
+  Proof. unfold_at; move => r1 r2 HR/=. solve_proper. Qed.
 
   #[global] Instance _at_persistent {P base} : Persistent P -> Persistent (_at base P).
   Proof. rewrite _at_eq. apply _. Qed.
@@ -411,144 +367,144 @@ Section with_cpp.
   Proof. rewrite _at_eq. apply _. Qed.
   #[global] Instance _at_timeless {P base} : Timeless P -> Timeless (_at base P).
   Proof. rewrite _at_eq. apply _. Qed.
-  #[global] Instance _at_laterable p (P : Rep) : Laterable P → Laterable (_at p P).
+  #[global] Instance _at_laterable p (P : Rep) : Laterable P → Laterable (p |-> P).
   Proof. rewrite _at_eq. apply _. Qed.
 
   Lemma Rep_equiv_at (P Q : Rep)
-    (HPQ : forall p : ptr, _at p P -|- _at p Q) :
+    (HPQ : forall p : ptr, p |-> P -|- p |-> Q) :
     P -|- Q.
-  Proof. constructor => p. move: HPQ => /(_ p). by rewrite _at_eq. Qed.
+  Proof. constructor => p. move: HPQ => /(_ p). by rewrite !_at_eq/_at_def => ->. Qed.
 
   Lemma Rep_entails_at (P Q : Rep)
-    (HPQ : forall p : ptr, _at p P |-- _at p Q) :
+    (HPQ : forall p : ptr, p |-> P |-- p |-> Q) :
     P |-- Q.
-  Proof. constructor => p. move: HPQ => /(_ p). by rewrite _at_eq. Qed.
+  Proof. constructor => p. move: HPQ => /(_ p). by rewrite !_at_eq. Qed.
   (* Inverses of [Rep_equiv_at] and [Rep_entails_at] are [Proper] instances [_at_proper] and [_at_mono], applicable via [f_equiv] or [apply]. *)
 
-  Lemma _at_as_Rep (l : ptr) (Q : ptr → mpred) : _at l (as_Rep Q) ⊣⊢ Q l.
-  Proof. by rewrite _at_eq/_at_def. Qed.
+  Lemma _at_as_Rep  p  (Q : ptr → mpred) : p |-> (as_Rep Q) ⊣⊢ Q p.
+  Proof. by rewrite _at_eq. Qed.
 
   (* Prefer [_at_as_Rep] *)
-  Lemma _at_loc p R : _at p R -|- R p.
-  Proof. by rewrite _at_eq/_at_def. Qed.
+  Lemma _at_loc p (R : Rep) : p |-> R -|- R p.
+  Proof. by rewrite _at_eq. Qed.
 
-  Lemma _at_emp l : _at l emp -|- emp.
+  Lemma _at_emp p : p |-> emp -|- emp.
   Proof. by rewrite _at_loc monPred_at_emp. Qed.
 
-  Lemma _at_exists l {T} (P : T -> Rep) :
-      _at l (Exists v : T, P v) -|- Exists v, _at l (P v).
+  Lemma _at_exists p {T} (P : T -> Rep) :
+      p |-> (Exists v : T, P v) -|- Exists v, p |-> (P v).
   Proof. by rewrite _at_loc monPred_at_exist; setoid_rewrite _at_loc. Qed.
 
-  Lemma _at_forall (l : ptr) T (P : T -> Rep) :
-    _at l (Forall x, P x) -|- Forall x, _at l (P x).
+  Lemma _at_forall p T (P : T -> Rep) :
+    p |-> (Forall x, P x) -|- Forall x, p |-> (P x).
   Proof. by rewrite _at_loc monPred_at_forall; setoid_rewrite _at_loc. Qed.
 
-  Lemma _at_only_provable l P :
-      _at l [| P |] -|- [| P |].
+  Lemma _at_only_provable p P :
+      p |-> [| P |] -|- [| P |].
   Proof. by rewrite _at_loc monPred_at_only_provable. Qed.
 
-  Lemma _at_pure (l : ptr) (P : Prop) :
-      _at l [! P !] -|- [! P !].
+  Lemma _at_pure  p  (P : Prop) :
+      p |-> [! P !] -|- [! P !].
   Proof. by rewrite _at_loc monPred_at_pure. Qed.
 
-  Lemma _at_sep (l : ptr) (P Q : Rep) :
-      _at l (P ** Q) -|- _at l P ** _at l Q.
+  Lemma _at_sep  p  (P Q : Rep) :
+      p |-> (P ** Q) -|- p |-> P ** p |-> Q.
   Proof. by rewrite !_at_loc monPred_at_sep. Qed.
 
-  Lemma _at_and (l : ptr) (P Q : Rep) :
-      _at l (P //\\ Q) -|- _at l P //\\ _at l Q.
+  Lemma _at_and  p  (P Q : Rep) :
+      p |-> (P //\\ Q) -|- p |-> P //\\ p |-> Q.
   Proof. by rewrite !_at_loc monPred_at_and. Qed.
 
-  Lemma _at_or (l : ptr) (P Q : Rep) :
-      _at l (P \\// Q) -|- _at l P \\// _at l Q.
+  Lemma _at_or  p  (P Q : Rep) :
+      p |-> (P \\// Q) -|- p |-> P \\// p |-> Q.
   Proof. by rewrite !_at_loc monPred_at_or. Qed.
 
-  Lemma _at_wand (l : ptr) (P Q : Rep) :
-      _at l (P -* Q) -|- _at l P -* _at l Q.
+  Lemma _at_wand  p  (P Q : Rep) :
+      p |-> (P -* Q) -|- p |-> P -* p |-> Q.
   Proof. by rewrite !_at_loc Rep_wand_force. Qed.
 
-  Lemma _at_pers (l : ptr) R : _at l (<pers> R) -|- <pers> _at l R.
+  Lemma _at_pers  p  R : p |-> (<pers> R) -|- <pers> p |-> R.
   Proof. by rewrite !_at_loc monPred_at_persistently. Qed.
 
-  Lemma _at_bupd (l : ptr) R : _at l (|==> R) -|- |==> _at l R.
+  Lemma _at_bupd  p  R : p |-> (|==> R) -|- |==> p |-> R.
   Proof. by rewrite !_at_loc monPred_at_bupd. Qed.
 
-  Lemma _at_fupd (l : ptr) R E1 E2 : _at l (|={E1,E2}=> R) -|- |={E1,E2}=> _at l R.
+  Lemma _at_fupd  p  R E1 E2 : p |-> (|={E1,E2}=> R) -|- |={E1,E2}=> p |-> R.
   Proof. by rewrite !_at_loc monPred_at_fupd. Qed.
 
-  Lemma _at_intuitionistically l (R : Rep) : _at l (□ R) ⊣⊢ □ (_at l R).
-  Proof. by rewrite _at_eq/_at_def monPred_at_intuitionistically. Qed.
-  Lemma _at_intuitionistically_if p b R : _at p (□?b R) -|- □?b (_at p R).
+  Lemma _at_intuitionistically  p  (R : Rep) : p |-> □ R ⊣⊢ □ (p |-> R).
+  Proof. by rewrite !_at_eq/_at_def; rewrite monPred_at_intuitionistically. Qed.
+  Lemma _at_intuitionistically_if (p : ptr) b R : p |-> (□?b R) -|- □?b (p |-> R).
   Proof. destruct b => //=. by rewrite _at_intuitionistically. Qed.
 
-  Lemma _at_except_0 p R : _at p (bi_except_0 R) -|- bi_except_0 (_at p R).
-  Proof. by rewrite _at_eq/_at_def monPred_at_except_0. Qed.
+  Lemma _at_except_0 (p : ptr) R : p |-> bi_except_0 R -|- bi_except_0 (p |-> R).
+  Proof. by rewrite !_at_eq/_at_def monPred_at_except_0. Qed.
 
-  Lemma _at_affinely (p : ptr) R : _at p (<affine> R) -|- <affine> _at p R.
-  Proof. by rewrite _at_eq/_at_def monPred_at_affinely. Qed.
+  Lemma _at_affinely (p : ptr) R : p |-> <affine> R -|- <affine> p |-> R.
+  Proof. by rewrite !_at_eq/_at_def monPred_at_affinely. Qed.
 
-  Lemma _at_affinely_if b (p : ptr) R : _at p (<affine>?b R) -|- <affine>?b _at p R.
-  Proof. by destruct b => //; rewrite _at_eq/_at_def monPred_at_affinely. Qed.
+  Lemma _at_affinely_if b (p : ptr) R : p |-> <affine>?b R -|- <affine>?b p |-> R.
+  Proof. by destruct b => //; rewrite !_at_eq/_at_def monPred_at_affinely. Qed.
 
-  Lemma _at_later p R : _at p (|> R) -|- |> _at p R.
-  Proof. by rewrite _at_eq/_at_def monPred_at_later. Qed.
+  Lemma _at_later p R : p |-> |> R -|- |> p |-> R.
+  Proof. by rewrite !_at_eq/_at_def; rewrite monPred_at_later. Qed.
 
-  Lemma _at_offsetR (l : ptr) (o : offset) (r : Rep) :
-      _at l (_offsetR o r) -|- _at (_offset_ptr l o) r.
-  Proof. by rewrite !_at_loc /flip _offsetR_eq/_offsetR_def /=. Qed.
+  Lemma _at_offsetR  p  (o : offset) (r : Rep) :
+      _at p (_offsetR o r) -|- _at (p ,, o) r.
+  Proof. rewrite !_at_loc /flip. by unfold_at. Qed.
 
-  Lemma _at_sepSPs l (xs : list Rep) : _at l ([∗] xs) -|- [∗] map (_at l) xs.
+  Lemma _at_sepSPs p (xs : list Rep) : p |-> ([∗] xs) -|- [∗] map (_at p) xs.
   Proof.
     induction xs => /=.
     - by rewrite _at_emp.
     - by rewrite _at_sep IHxs.
   Qed.
 
-  Lemma _at_big_sepL A l : forall (xs : list A) (Φ : nat -> A -> Rep),
-      _at l ([∗ list] i↦x∈xs, Φ i x) -|- ([∗ list] i↦x∈xs, _at l (Φ i x)).
+  Lemma _at_big_sepL A p : forall (xs : list A) (Φ : nat -> A -> Rep),
+      p |-> ([∗ list] i↦x∈xs, Φ i x) -|- ([∗ list] i↦x∈xs, p |-> (Φ i x)).
   Proof.
     elim => /=.
     - move => ?; by rewrite _at_emp.
     - move => x xs IH ?. by rewrite _at_sep IH.
   Qed.
 
-  #[global] Instance _at_fractional (r : Qp → Rep) (l : ptr) `{!Fractional r} :
-    Fractional (λ q, _at l (r q)).
+  #[global] Instance _at_fractional (r : Qp → Rep)  p  `{!Fractional r} :
+    Fractional (λ q, p |-> (r q)).
   Proof.
     intros q1 q2; by rewrite fractional _at_sep.
   Qed.
-  #[global] Instance _at_as_fractional (r : Qp → Rep) q (l : ptr)
+  #[global] Instance _at_as_fractional (r : Qp → Rep) q  p
       `{!AsFractional (r q) r q} :
-    AsFractional (_at l (r q)) (λ q, _at l (r q)) q.
+    AsFractional (_at p (r q)) (λ q, _at p (r q)) q.
   Proof. constructor. done. apply _. Qed.
 
   #[global] Instance _at_observe {p} {Q R : Rep} :
     Observe Q R ->
-    Observe (_at p Q) (_at p R).
+    Observe (p |-> Q) (p |-> R).
   Proof. move->. by rewrite /Observe _at_pers. Qed.
 
   #[global] Instance _at_observe_2 {p} {Q R1 R2 : Rep} :
     Observe2 Q R1 R2 ->
-    Observe2 (_at p Q) (_at p R1) (_at p R2).
+    Observe2 (p |-> Q) (p |-> R1) (p |-> R2).
   Proof. move->. by rewrite /Observe2 _at_wand _at_pers. Qed.
 
   #[global] Instance _at_observe_only_provable Q p (R : Rep) :
-    Observe [| Q |] R → Observe [| Q |] (_at p R).
+    Observe [| Q |] R → Observe [| Q |] (p |-> R).
   Proof. rewrite -_at_only_provable. apply _. Qed.
   #[global] Instance _at_observe_2_only_provable Q p (R1 R2 : Rep) :
-    Observe2 [| Q |] R1 R2 → Observe2 [| Q |] (_at p R1) (_at p R2).
+    Observe2 [| Q |] R1 R2 → Observe2 [| Q |] (p |-> R1) (p |-> R2).
   Proof. rewrite -_at_only_provable. apply _. Qed.
 
-  #[global] Instance _at_observe_pure Q l (R : Rep) :
-    Observe [! Q !] R → Observe [! Q !] (_at l R).
+  #[global] Instance _at_observe_pure Q p (R : Rep) :
+    Observe [! Q !] R → Observe [! Q !] (p |-> R).
   Proof. rewrite -_at_pure. apply _. Qed.
-  #[global] Instance _at_observe_2_pure Q l (R1 R2 : Rep) :
-    Observe2 [! Q !] R1 R2 → Observe2 [! Q !] (_at l R1) (_at l R2).
+  #[global] Instance _at_observe_2_pure Q p (R1 R2 : Rep) :
+    Observe2 [! Q !] R1 R2 → Observe2 [! Q !] (p |-> R1) (p |-> R2).
   Proof. rewrite -_at_pure. apply _. Qed.
 
-  Lemma _at_obs (l : ptr) (r : Rep) P :
+  Lemma _at_obs  p  (r : Rep) P :
     r |-- r ** [| P |] →
-    _at l r |-- _at l r ** [| P |].
+    p |-> r |-- p |-> r ** [| P |].
   Proof. intros. apply observe_elim, _at_observe_only_provable. exact: observe_intro. Qed.
 
   #[global] Instance pureR_ne : NonExpansive pureR.
@@ -687,7 +643,7 @@ Section with_cpp.
   Lemma _at_pureR x (P : mpred) : _at x (pureR P) -|- P.
   Proof. by rewrite !_at_loc /pureR. Qed.
 
-  Lemma _offsetR_pureR o P : _offsetR o (pureR P) -|- pureR P.
+  Lemma _offsetR_pureR o P : o |-> (pureR P) -|- pureR P.
   Proof. by apply Rep_equiv_at => p; rewrite _at_offsetR !_at_pureR. Qed.
 
   (** As this isn't syntax-directed, we conservatively avoid
@@ -695,13 +651,15 @@ Section with_cpp.
       observations). It's handy under [#[local] Existing Instance
       _at_observe_pureR] to project a [pureR Q] conjunct out of
       representation predicates. *)
-  Lemma _at_observe_pureR Q (l : ptr) (R : Rep) :
-    Observe (pureR Q) R → Observe Q (_at l R).
+  Lemma _at_observe_pureR Q  p  (R : Rep) :
+    Observe (pureR Q) R → Observe Q (p |-> R).
   Proof.
     rewrite /Observe=>->. rewrite -pureR_persistently _at_pureR. done.
   Qed.
 
 End with_cpp.
 
-#[global] Typeclasses Opaque _at _offsetR pureR as_Rep.
-#[global] Opaque _at _offsetR.
+#[global] Typeclasses Opaque pureR as_Rep.
+
+Export rep_defs.
+Export heap_notations.
