theories/lang/cpp/logic/arr.v
@@ -21,8 +21,6 @@ From bedrock.lang.cpp.semantics Require Import values.
 #[local] Arguments N.of_nat _ : simpl never.
 #[local] Arguments N.to_nat _ : simpl never.
 
-#[local] Arguments _offsetR {_ _} _ _%bi_scope.
-
 Lemma size_of_array_0_Some σ ty :
   is_Some (size_of σ ty) → size_of σ (Tarray ty 0) = Some 0%N.
 Proof. by move=>[]sz /= ->. Qed.
@@ -42,10 +40,12 @@ End simpl_never.
 (** PDS: Misplaced *)
 Section offsetR.
   Context `{Σ : cpp_logic}.
+  Import heap_notations.INTERNAL.
+  Ltac unfold_dot := rewrite /DOT_dot/= !_dot.unlock.
 
-  Lemma monPred_at_offsetR offs R p :
-    (_offsetR offs R) p -|- R (p ., offs).
-  Proof. by rewrite _offsetR_eq. Qed.
+  Lemma monPred_at_offsetR offs (R : Rep) (p : ptr) :
+    (_offsetR offs R) p -|- R (p ,, offs).
+  Proof. by rewrite _offsetR_eq; unfold_dot. Qed.
 End offsetR.
 
 Implicit Types (p : ptr) (σ : genv).
@@ -97,23 +97,26 @@ Section validR.
 
   Lemma _at_sub_0 p ty R
     (Hsz : is_Some (size_of resolve ty)) :
-    p ., (.[ ty ! 0 ]) |-> R -|- p |-> R.
+    p ,, (.[ ty ! 0 ]) |-> R -|- p |-> R.
   Proof. by rewrite offset_ptr_sub_0. Qed.
 
+  Lemma at_offsetR (l : ptr) (o : offset) (r : Rep) : l |-> o |-> r -|- l ,, o |-> r.
+  Proof. by rewrite _at_offsetR. Qed.
+
   Lemma _at_sub_sub p ty a b R :
-    p ., (.[ ty ! a ]) |-> (.[ ty ! b ] |-> R) ⊣⊢
-    p ., (.[ ty ! a + b ]) |-> R.
-  Proof. by rewrite -!_at_offsetR _offsetR_sub_sub. Qed.
+    p ,, (.[ ty ! a ]) |-> (.[ ty ! b ] |-> R) ⊣⊢
+    p ,, (.[ ty ! a + b ]) |-> R.
+  Proof. by rewrite -!at_offsetR _offsetR_sub_sub. Qed.
 
   Lemma _at_succ_sub p ty z R :
-    p ., (.[ ty ! 1 ]) |-> (.[ ty ! z ] |-> R) ⊣⊢
-    p ., (.[ ty ! Z.succ z]) |-> R.
-  Proof. by rewrite -!_at_offsetR _offsetR_succ_sub. Qed.
+    p ,, (.[ ty ! 1 ]) |-> (.[ ty ! z ] |-> R) ⊣⊢
+    p ,, (.[ ty ! Z.succ z]) |-> R.
+  Proof. by rewrite -!at_offsetR _offsetR_succ_sub. Qed.
 
   Lemma _at_sub_succ p ty z R :
-    p ., (.[ ty ! z ]) |-> (.[ ty ! 1 ] |-> R) ⊣⊢
+    p ,, (.[ ty ! z ]) |-> (.[ ty ! 1 ] |-> R) ⊣⊢
     p .[ ty ! Z.succ z] |-> R.
-  Proof. by rewrite -!_at_offsetR _offsetR_sub_succ. Qed.
+  Proof. by rewrite -!at_offsetR _offsetR_sub_succ. Qed.
 End validR.
 
 Definition arrR_def `{Σ : cpp_logic} {σ : genv} (ty : type) (Rs : list Rep) : Rep :=
@@ -181,25 +184,48 @@ Section arrR.
   #[global] Instance arrR_valid_end ty Rs : Observe (.[ ty ! length Rs ] |-> validR) (arrR ty Rs).
   Proof. rewrite arrR_eq /arrR_def /=. refine _. Qed.
 
+  Lemma offsetR_sub_0 (ty : type) (R : Rep) (_ : is_Some (size_of σ ty)) : .[ ty ! 0 ] |-> R -|- R.
+  Proof. by rewrite _offsetR_sub_0. Qed.
+
   Lemma arrR_nil ty : arrR ty [] -|- validR ** [| is_Some (size_of σ ty) |].
   Proof.
     rewrite arrR_eq /arrR_def /= right_id.
     apply: (observe_both (is_Some (size_of σ ty))).
-    intro. by rewrite _offsetR_sub_0.
+    intro. by rewrite offsetR_sub_0.
   Qed.
+
+  Lemma offsetR_sep (o : offset) (r1 r2 : Rep) :
+    o |-> (r1 ** r2) -|- o |-> r1 ** o |-> r2.
+  Proof. by apply _offsetR_sep. Qed.
+
+  Lemma offsetR_only_provable (o : offset) (P : Prop) : o |-> [| P |] -|- [| P |].
+  Proof. by apply _offsetR_only_provable. Qed.
+
+  Lemma offsetR_observe (o : offset) (Q R : Rep) (_ : Observe Q R) : Observe (o |-> Q) (o |-> R).
+  Proof. by apply _offsetR_observe. Qed.
+
+  Lemma offsetR_big_sepL (o : offset) (T : Type) (Rs : list T) (F : nat -> T -> Rep) :
+    o |-> ([∗ list] i↦x ∈ Rs, F i x) -|- ([∗ list] i↦x ∈ Rs, o |-> F i x).
+  Proof. apply _offsetR_big_sepL. Qed.
 
   Lemma arrR_cons ty R Rs :
     arrR ty (R :: Rs) -|- type_ptrR ty ** R ** .[ ty ! 1 ] |-> arrR ty Rs.
   Proof.
-    rewrite arrR_eq/arrR_def /= !_offsetR_sep !_offsetR_only_provable.
+    rewrite arrR_eq/arrR_def /= !offsetR_sep !offsetR_only_provable.
     apply: (observe_both (is_Some (size_of σ ty))) => Hsz.
-    rewrite !_offsetR_sub_0 // _offsetR_big_sepL -assoc.
+    rewrite !offsetR_sub_0 // offsetR_big_sepL -assoc.
     rewrite _offsetR_succ_sub Nat2Z.inj_succ;
       setoid_rewrite _offsetR_succ_sub; setoid_rewrite Nat2Z.inj_succ.
     iSplit; [ iIntros "(? & ? & ? & ? & ?)" | iIntros "(? & ? & ? & _ & ?)"];
      by iFrame.
   Qed.
 
+  Lemma offsetR_id (R : Rep) : o_id |-> R -|- R.
+  Proof. by apply _offsetR_id. Qed.
+
+  Lemma offsetR_sub_sub (ty : type) (a b : Z) (R : Rep) :
+    .[ ty ! a ] |-> .[ ty ! b ] |-> R -|- .[ ty ! a + b ] |-> R.
+  Proof. by apply _offsetR_sub_sub. Qed.
 
   Lemma arrR_valid_obs ty Rs (i : Z) (Hi : (0 ≤ i ≤ Z.of_nat (length Rs))%Z) :
     Observe (.[ ty ! i ] |-> validR) (arrR ty Rs).
@@ -209,13 +235,13 @@ Section arrR.
     generalize dependent i.
     induction Rs => i Hi /=; [ rewrite arrR_nil | rewrite arrR_cons ].
     { simpl in *; have ->:i = 0; first lia.
-      rewrite o_sub_0 // _offsetR_id. iIntros "[#$ $]". }
+      rewrite o_sub_0 // offsetR_id. iIntros "[#$ $]". }
     { case (decide (0 < i)%Z) => Hlt.
       { rewrite {1}(IHRs (i -1)%Z); last by simpl in *; split; lia.
-        rewrite _offsetR_sep _offsetR_sub_sub. iIntros "($ & $ & $ & x)".
+        rewrite offsetR_sep offsetR_sub_sub. iIntros "($ & $ & $ & x)".
         iStopProof. f_equiv. f_equiv. lia. }
       { have ->: i = 0; first by lia.
-        rewrite -svalidR_validR -type_ptrR_svalidR _offsetR_sub_0 //.
+        rewrite -svalidR_validR -type_ptrR_svalidR offsetR_sub_0 //.
         iIntros "(#$ & $ & $)". } }
   Qed.
 
@@ -226,20 +252,24 @@ Section arrR.
     { rewrite arrR_cons. rewrite type_ptrR_svalidR svalidR_validR; refine _. }
   Qed.
 
+  Lemma offsetR_succ_sub (ty : type) (z : Z) (R : Rep) :
+    .[ ty ! 1 ] |-> .[ ty ! z ] |-> R -|- .[ ty ! Z.succ z ] |-> R.
+  Proof. apply _offsetR_succ_sub. Qed.
+
   Lemma arrR_append ty ys xs :
     arrR ty (xs ++ ys) -|- arrR ty xs ** .[ ty ! length xs ] |-> arrR ty ys.
   Proof.
     induction xs => /=.
     { apply: (observe_both (is_Some _)) => Hsz.
-      rewrite arrR_nil /= o_sub_0 // _offsetR_id.
+      rewrite arrR_nil /= o_sub_0 // offsetR_id.
       iSplit; last iIntros "[_ $]". iIntros "X"; repeat iSplit => //.
       iApply (observe with "X"). }
-    { by rewrite !arrR_cons IHxs !_offsetR_sep !_offsetR_succ_sub Nat2Z.inj_succ -!assoc. }
+    { by rewrite !arrR_cons IHxs !offsetR_sep !offsetR_succ_sub Nat2Z.inj_succ -!assoc. }
   Qed.
 
   Lemma arrR_singleton ty R : arrR ty [R] -|- type_ptrR ty ** R.
   Proof.
-    rewrite arrR_cons arrR_nil _offsetR_sep _offsetR_only_provable.
+    rewrite arrR_cons arrR_nil offsetR_sep offsetR_only_provable.
     iSplit.
     { iIntros "($ & $ & _ & %)". }
     { iIntros "(#tp & $)". rewrite -type_ptrR_validR_plus_one.
@@ -297,12 +327,24 @@ Section array.
     arrayR ty R (xs ++ [y]) -|- arrayR ty R xs ** .[ ty ! length xs ] |-> (type_ptrR ty ** R y).
   Proof. by rewrite arrayR_eq /arrayR_def fmap_app arrR_snoc fmap_length. Qed.
 
+  Lemma at_sep (l : ptr) (P Q : Rep) : l |-> (P ** Q) -|- l |-> P ** l |-> Q.
+  Proof. apply _at_sep. Qed.
+
+  Lemma at_wand (l : ptr) (P Q : Rep) : l |-> (P -* Q) -|- l |-> P -* l |-> Q.
+  Proof. apply _at_wand. Qed.
+
+  Lemma at_pure (l : ptr) (P : Prop) : l |-> ⌜P⌝ -|- ⌜P⌝.
+  Proof. apply _at_pure. Qed.
+
+  Lemma at_pureR (x : ptr) (P : mpred) : (x |-> pureR P)%stdpp -|- P.
+  Proof. apply _at_pureR. Qed.
+
   Lemma arrayR_snoc_obs p xs y
         `{Hobs : ∀ x, Observe (type_ptrR ty) (R x)} :
         p |-> arr.arrayR ty R (xs ++ [y])
-    -|- p |-> arr.arrayR ty R xs ** p ., (.[ty ! Z.of_nat (length xs)]) |-> R y.
+    -|- p |-> arr.arrayR ty R xs ** p ,, (.[ty ! Z.of_nat (length xs)]) |-> R y.
   Proof.
-    rewrite arrayR_snoc !_at_sep !_at_offsetR _at_sep. f_equiv.
+    rewrite arrayR_snoc !at_sep !at_offsetR at_sep. f_equiv.
     rewrite (comm bi_sep).
     exact: observe_equiv.
   Qed.
@@ -319,9 +361,9 @@ Section array.
     elim: xs i Hlen => [|x xs IHxs] [|i] /= Hlen; try lia;
                         rewrite arrayR_cons.
     { apply: (observe_lhs (is_Some (size_of resolve ty))) => Hsz.
-      rewrite o_sub_0 // _offsetR_id. iDestruct 1 as "[$ _]". }
+      rewrite o_sub_0 // offsetR_id. iDestruct 1 as "[$ _]". }
     { rewrite (IHxs i); try lia.
-      rewrite _offsetR_succ_sub Nat2Z.inj_succ.
+      rewrite offsetR_succ_sub Nat2Z.inj_succ.
       iDestruct 1 as "(_ & _ & $)". }
   Qed.
 
@@ -332,19 +374,23 @@ Section array.
     intros []. have := arrayR_sub_type_ptr_nat_obs (Z.to_nat i) xs.
     rewrite Z2Nat.id //. apply. lia.
   Qed.
+Check @_at_observe.
+
+  Lemma at_observe p (Q P : Rep) (_ : Observe Q P) : Observe (p |-> Q) (p |-> P).
+  Proof. by apply _at_observe. Qed.
 
   Lemma _at_arrayR_sub_type_ptrR_nat_obs (i : nat) p xs
         (Hlen : i < length xs) :
     Observe (p .[ ty ! i ] |-> type_ptrR ty) (p |-> arrayR ty R xs).
   Proof.
-    rewrite -_at_offsetR //. by apply _at_observe, arrayR_sub_type_ptr_nat_obs.
+    rewrite -at_offsetR //. by apply at_observe, arrayR_sub_type_ptr_nat_obs.
   Qed.
 
   Lemma _at_arrayR_sub_type_ptrR_obs (i : Z) p xs
         (Hlen : (0 ≤ i < Z.of_nat $ length xs)%Z) :
     Observe (p .[ ty ! i ] |-> type_ptrR ty) (p |-> arrayR ty R xs).
   Proof.
-    rewrite -_at_offsetR //. by apply _at_observe, arrayR_sub_type_ptr_obs.
+    rewrite -at_offsetR //. by apply at_observe, arrayR_sub_type_ptr_obs.
   Qed.
 
   Lemma arrayR_sub_svalidR_obs (i : Z) xs  :
@@ -369,8 +415,8 @@ Section array.
         (Hi : i ≤ length xs) :
     Observe (p .[ ty ! i ] |-> validR) (p |-> arrayR ty R xs).
   Proof.
-    rewrite -_at_offsetR.
-    by apply _at_observe, arrayR_valid_obs.
+    rewrite -at_offsetR.
+    by apply at_observe, arrayR_valid_obs.
   Qed.
 
   #[global] Instance arrayR_valid_base_obs {xs} : Observe validR (arrayR ty R xs).
@@ -431,7 +477,7 @@ Section array.
            _sub ty (iZ + 1) |-> arrayR ty R (drop (S i) xs).
   Proof.
     intros Hi Hl.
-    rewrite -{1}(take_drop_middle xs i _ Hl) arrayR_app arrayR_cons !_offsetR_sep.
+    rewrite -{1}(take_drop_middle xs i _ Hl) arrayR_app arrayR_cons !offsetR_sep.
     f_equiv.
     enough (length (take i xs) = i) as ->.
     { subst. by rewrite _offsetR_sub_sub. }
@@ -448,7 +494,7 @@ Proof.
   red. intros.
   induction l.
   { rewrite !arrayR_nil. iSplit; eauto. iIntros "[[#a b] _]"; eauto. }
-  { rewrite !arrayR_cons IHl H !_offsetR_sep. iSplit.
+  { rewrite !arrayR_cons IHl H !offsetR_sep. iSplit.
     { iIntros "(#a & [b c] & d & e)"; iFrame "∗#". }
     { iIntros "([a [b c]] & [_ [e f]])"; iFrame. } }
 Qed.
